\begin{displaymath}
f(t) = U_{0}(t)sin(\pi t) -  U_{1}(t)sin(\pi t)
\end{displaymath}
\begin{displaymath}
f(t) = sin(\pi t) +  U_{1}(t)sin(\pi (t-1))
\end{displaymath}

\end{frame}
%=======================================================%
\begin{frame}
\frametitle{Laplace Transforms}
\Large

\begin{displaymath}
F(s) = \frac{1-e^{-s}-se^{-s}}{s^2} \times \frac{1}{1-e^{-s}}
\end{displaymath}
\begin{displaymath}
F(s) = G(s) \times \frac{1}{1-e^{-ps}}
\end{displaymath}

\end{frame}
%=======================================================%
\begin{frame}
\frametitle{Laplace Transforms}
\Large

\begin{displaymath}
F(s) = G(s) \times \frac{1}{1-e^{-ps}}
\end{displaymath}
\begin{displaymath}
f(t) = (2t) - U_{1}(t).(2t) +  U_{1}(t).(4) - U_{1}(t).(2t) - U_{2}(t).(4-2t)
\end{displaymath}
\end{frame}
%=======================================================%
\begin{frame}
\frametitle{Laplace Transforms}
\Large

\begin{displaymath}
f(t) = [U_{0}(t)-U_{1}(t) ]\times (2t) +  [U_{1}(t)-U_{2}(t) ]\times (4-2t)
\end{displaymath}
\begin{displaymath}
f(t) = U_{0}(t).(2t) - U_{1}(t).(2t) +  U_{1}(t).(4-2t) - U_{2}(t).(4-2t)
\end{displaymath}
\begin{displaymath}
f(t) = (2t) - U_{1}(t).[4 \times (t-1)] - U_{2}(t).[-2 \times (t-2)]
\end{displaymath}
\begin{displaymath}
F(s) = \frac{2}{s^2} - e^{-s}\frac{4}{s^2} + e^{-2s}\frac{2}{s^2}
\end{displaymath}
\end{frame}
%=======================================================%
\begin{frame}
\frametitle{Laplace Transforms}
\Large
